<?xml version="1.0"?>
<rdf:RDF xmlns="http://www.hsu-ifa.de/ontologies/WADL#"
     xml:base="http://www.hsu-ifa.de/ontologies/WADL"
     xmlns:owl="http://www.w3.org/2002/07/owl#"
     xmlns:rdf="http://www.w3.org/1999/02/22-rdf-syntax-ns#"
     xmlns:xml="http://www.w3.org/XML/1998/namespace"
     xmlns:xsd="http://www.w3.org/2001/XMLSchema#"
     xmlns:WADL="http://www.hsu-ifa.de/ontologies/WADL#"
     xmlns:rdfs="http://www.w3.org/2000/01/rdf-schema#">
    <owl:Ontology rdf:about="http://www.w3id.org/hsu-aut/WADL">
        <owl:versionIRI rdf:resource="http://www.w3id.org/hsu-aut/WADL/2.0.0"/>
        <owl:versionInfo>2.0.0</owl:versionInfo>
    </owl:Ontology>
    


    <!-- 
    ///////////////////////////////////////////////////////////////////////////////////////
    //
    // Object Properties
    //
    ///////////////////////////////////////////////////////////////////////////////////////
     -->

    


    <!-- http://www.w3id.org/hsu-aut/WADL#hasMethod -->

    <owl:ObjectProperty rdf:about="http://www.w3id.org/hsu-aut/WADL#hasMethod">
        <rdfs:domain rdf:resource="http://www.w3id.org/hsu-aut/WADL#Resource"/>
        <rdfs:range rdf:resource="http://www.w3id.org/hsu-aut/WADL#Method"/>
    </owl:ObjectProperty>
    


    <!-- http://www.w3id.org/hsu-aut/WADL#hasOntologicalParameterType -->

    <owl:ObjectProperty rdf:about="http://www.w3id.org/hsu-aut/WADL#hasOntologicalParameterType">
        <owl:inverseOf rdf:resource="http://www.w3id.org/hsu-aut/WADL#isOntologicalParameterTypeFor"/>
        <rdfs:domain rdf:resource="http://www.w3id.org/hsu-aut/WADL#Parameter"/>
        <rdfs:range rdf:resource="http://www.w3.org/2002/07/owl#Thing"/>
        <rdfs:comment>This object property is used to declare another individual as the data type of the parameter.</rdfs:comment>
    </owl:ObjectProperty>
    


    <!-- http://www.w3id.org/hsu-aut/WADL#hasParameter -->

    <owl:ObjectProperty rdf:about="http://www.w3id.org/hsu-aut/WADL#hasParameter">
        <rdfs:domain>
            <owl:Class>
                <owl:unionOf rdf:parseType="Collection">
                    <rdf:Description rdf:about="http://www.w3id.org/hsu-aut/WADL#Representation"/>
                    <rdf:Description rdf:about="http://www.w3id.org/hsu-aut/WADL#Request"/>
                    <rdf:Description rdf:about="http://www.w3id.org/hsu-aut/WADL#Resource"/>
                    <rdf:Description rdf:about="http://www.w3id.org/hsu-aut/WADL#Response"/>
                </owl:unionOf>
            </owl:Class>
        </rdfs:domain>
        <rdfs:range rdf:resource="http://www.w3id.org/hsu-aut/WADL#Parameter"/>
    </owl:ObjectProperty>
    


    <!-- http://www.w3id.org/hsu-aut/WADL#hasParameterOption -->

    <owl:ObjectProperty rdf:about="http://www.w3id.org/hsu-aut/WADL#hasParameterOption">
        <rdfs:domain rdf:resource="http://www.w3id.org/hsu-aut/WADL#Parameter"/>
        <rdfs:range rdf:resource="http://www.w3id.org/hsu-aut/WADL#Option"/>
    </owl:ObjectProperty>
    


    <!-- http://www.w3id.org/hsu-aut/WADL#hasRepresentation -->

    <owl:ObjectProperty rdf:about="http://www.w3id.org/hsu-aut/WADL#hasRepresentation">
        <rdfs:domain>
            <owl:Class>
                <owl:unionOf rdf:parseType="Collection">
                    <rdf:Description rdf:about="http://www.w3id.org/hsu-aut/WADL#Request"/>
                    <rdf:Description rdf:about="http://www.w3id.org/hsu-aut/WADL#Response"/>
                </owl:unionOf>
            </owl:Class>
        </rdfs:domain>
        <rdfs:range rdf:resource="http://www.w3id.org/hsu-aut/WADL#Representation"/>
    </owl:ObjectProperty>
    


    <!-- http://www.w3id.org/hsu-aut/WADL#hasRequest -->

    <owl:ObjectProperty rdf:about="http://www.w3id.org/hsu-aut/WADL#hasRequest">
        <rdfs:domain rdf:resource="http://www.w3id.org/hsu-aut/WADL#Method"/>
        <rdfs:range rdf:resource="http://www.w3id.org/hsu-aut/WADL#Request"/>
    </owl:ObjectProperty>
    


    <!-- http://www.w3id.org/hsu-aut/WADL#hasResource -->

    <owl:ObjectProperty rdf:about="http://www.w3id.org/hsu-aut/WADL#hasResource">
        <rdfs:domain>
            <owl:Class>
                <owl:unionOf rdf:parseType="Collection">
                    <rdf:Description rdf:about="http://www.w3id.org/hsu-aut/WADL#Resource"/>
                    <rdf:Description rdf:about="http://www.w3id.org/hsu-aut/WADL#Resources"/>
                </owl:unionOf>
            </owl:Class>
        </rdfs:domain>
        <rdfs:range rdf:resource="http://www.w3id.org/hsu-aut/WADL#Resource"/>
    </owl:ObjectProperty>
    


    <!-- http://www.w3id.org/hsu-aut/WADL#hasResponse -->

    <owl:ObjectProperty rdf:about="http://www.w3id.org/hsu-aut/WADL#hasResponse">
        <rdfs:domain rdf:resource="http://www.w3id.org/hsu-aut/WADL#Method"/>
        <rdfs:range rdf:resource="http://www.w3id.org/hsu-aut/WADL#Response"/>
    </owl:ObjectProperty>
    


    <!-- http://www.w3id.org/hsu-aut/WADL#isOntologicalParameterTypeFor -->

    <owl:ObjectProperty rdf:about="http://www.w3id.org/hsu-aut/WADL#isOntologicalParameterTypeFor">
        <rdfs:domain rdf:resource="http://www.w3.org/2002/07/owl#Thing"/>
        <rdfs:range rdf:resource="http://www.w3id.org/hsu-aut/WADL#Parameter"/>
        <rdfs:comment>This object property is used to declare another individual as the data type of the parameter.</rdfs:comment>
    </owl:ObjectProperty>
    


    <!-- 
    ///////////////////////////////////////////////////////////////////////////////////////
    //
    // Data properties
    //
    ///////////////////////////////////////////////////////////////////////////////////////
     -->

    


    <!-- http://www.w3id.org/hsu-aut/WADL#hasBase -->

    <owl:DatatypeProperty rdf:about="http://www.w3id.org/hsu-aut/WADL#hasBase">
        <rdfs:domain rdf:resource="http://www.w3id.org/hsu-aut/WADL#Resources"/>
        <rdfs:range rdf:resource="http://www.w3.org/2001/XMLSchema#anyURI"/>
    </owl:DatatypeProperty>
    


    <!-- http://www.w3id.org/hsu-aut/WADL#hasId -->

    <owl:DatatypeProperty rdf:about="http://www.w3id.org/hsu-aut/WADL#hasId">
        <rdfs:domain>
            <owl:Class>
                <owl:unionOf rdf:parseType="Collection">
                    <rdf:Description rdf:about="http://www.w3id.org/hsu-aut/WADL#Method"/>
                    <rdf:Description rdf:about="http://www.w3id.org/hsu-aut/WADL#Parameter"/>
                    <rdf:Description rdf:about="http://www.w3id.org/hsu-aut/WADL#Representation"/>
                    <rdf:Description rdf:about="http://www.w3id.org/hsu-aut/WADL#Resource"/>
                </owl:unionOf>
            </owl:Class>
        </rdfs:domain>
        <rdfs:range rdf:resource="http://www.w3.org/2001/XMLSchema#string"/>
    </owl:DatatypeProperty>
    


    <!-- http://www.w3id.org/hsu-aut/WADL#hasMediaType -->

    <owl:DatatypeProperty rdf:about="http://www.w3id.org/hsu-aut/WADL#hasMediaType">
        <rdfs:domain>
            <owl:Class>
                <owl:unionOf rdf:parseType="Collection">
                    <rdf:Description rdf:about="http://www.w3id.org/hsu-aut/WADL#Option"/>
                    <rdf:Description rdf:about="http://www.w3id.org/hsu-aut/WADL#Representation"/>
                </owl:unionOf>
            </owl:Class>
        </rdfs:domain>
        <rdfs:range rdf:resource="http://www.w3.org/2000/01/rdf-schema#Literal"/>
    </owl:DatatypeProperty>
    


    <!-- http://www.w3id.org/hsu-aut/WADL#hasOptionValue -->

    <owl:DatatypeProperty rdf:about="http://www.w3id.org/hsu-aut/WADL#hasOptionValue">
        <rdfs:domain rdf:resource="http://www.w3id.org/hsu-aut/WADL#Option"/>
        <rdfs:range rdf:resource="http://www.w3.org/2001/XMLSchema#string"/>
    </owl:DatatypeProperty>
    


    <!-- http://www.w3id.org/hsu-aut/WADL#hasParameterDefault -->

    <owl:DatatypeProperty rdf:about="http://www.w3id.org/hsu-aut/WADL#hasParameterDefault">
        <rdfs:domain rdf:resource="http://www.w3id.org/hsu-aut/WADL#Parameter"/>
    </owl:DatatypeProperty>
    


    <!-- http://www.w3id.org/hsu-aut/WADL#hasParameterName -->

    <owl:DatatypeProperty rdf:about="http://www.w3id.org/hsu-aut/WADL#hasParameterName">
        <rdfs:domain rdf:resource="http://www.w3id.org/hsu-aut/WADL#Parameter"/>
        <rdfs:range rdf:resource="http://www.w3.org/2001/XMLSchema#NMTOKEN"/>
    </owl:DatatypeProperty>
    


    <!-- http://www.w3id.org/hsu-aut/WADL#hasParameterRequired -->

    <owl:DatatypeProperty rdf:about="http://www.w3id.org/hsu-aut/WADL#hasParameterRequired">
        <rdfs:domain rdf:resource="http://www.w3id.org/hsu-aut/WADL#Parameter"/>
        <rdfs:range rdf:resource="http://www.w3.org/2001/XMLSchema#boolean"/>
    </owl:DatatypeProperty>
    


    <!-- http://www.w3id.org/hsu-aut/WADL#hasParameterType -->

    <owl:DatatypeProperty rdf:about="http://www.w3id.org/hsu-aut/WADL#hasParameterType">
        <rdfs:domain rdf:resource="http://www.w3id.org/hsu-aut/WADL#Parameter"/>
        <rdfs:range rdf:resource="http://www.w3.org/2001/XMLSchema#string"/>
        <rdfs:comment>Optionally indicates the type of the parameter as an XML qualified name, defaults to xsd:string.</rdfs:comment>
    </owl:DatatypeProperty>
    


    <!-- http://www.w3id.org/hsu-aut/WADL#hasPath -->

    <owl:DatatypeProperty rdf:about="http://www.w3id.org/hsu-aut/WADL#hasPath">
        <rdfs:domain>
            <owl:Class>
                <owl:unionOf rdf:parseType="Collection">
                    <rdf:Description rdf:about="http://www.w3id.org/hsu-aut/WADL#Parameter"/>
                    <rdf:Description rdf:about="http://www.w3id.org/hsu-aut/WADL#Resource"/>
                </owl:unionOf>
            </owl:Class>
        </rdfs:domain>
        <rdfs:range rdf:resource="http://www.w3.org/2001/XMLSchema#string"/>
    </owl:DatatypeProperty>
    


    <!-- http://www.w3id.org/hsu-aut/WADL#hasQueryType -->

    <owl:DatatypeProperty rdf:about="http://www.w3id.org/hsu-aut/WADL#hasQueryType">
        <rdfs:domain rdf:resource="http://www.w3id.org/hsu-aut/WADL#Resource"/>
        <rdfs:range rdf:resource="http://www.w3.org/2001/XMLSchema#string"/>
    </owl:DatatypeProperty>
    


    <!-- 
    ///////////////////////////////////////////////////////////////////////////////////////
    //
    // Classes
    //
    ///////////////////////////////////////////////////////////////////////////////////////
     -->

    


    <!-- http://www.w3id.org/hsu-aut/WADL#DELETE -->

    <owl:Class rdf:about="http://www.w3id.org/hsu-aut/WADL#DELETE">
        <rdfs:subClassOf rdf:resource="http://www.w3id.org/hsu-aut/WADL#Method"/>
        <rdfs:comment>The DELETE method deletes the specified resource.</rdfs:comment>
    </owl:Class>
    


    <!-- http://www.w3id.org/hsu-aut/WADL#GET -->

    <owl:Class rdf:about="http://www.w3id.org/hsu-aut/WADL#GET">
        <rdfs:subClassOf rdf:resource="http://www.w3id.org/hsu-aut/WADL#Method"/>
        <rdfs:comment>The GET method requests a representation of the specified resource. Requests using GET should only retrieve data.</rdfs:comment>
    </owl:Class>
    


    <!-- http://www.w3id.org/hsu-aut/WADL#HEAD -->

    <owl:Class rdf:about="http://www.w3id.org/hsu-aut/WADL#HEAD">
        <rdfs:subClassOf rdf:resource="http://www.w3id.org/hsu-aut/WADL#Method"/>
        <rdfs:comment>The HEAD method asks for a response identical to that of a GET request, but without the response body.</rdfs:comment>
    </owl:Class>
    


    <!-- http://www.w3id.org/hsu-aut/WADL#HeaderParameter -->

    <owl:Class rdf:about="http://www.w3id.org/hsu-aut/WADL#HeaderParameter">
        <rdfs:subClassOf rdf:resource="http://www.w3id.org/hsu-aut/WADL#Parameter"/>
        <rdfs:comment>Specifies a HTTP header that pertains to the HTTP request (resource or request) or HTTP response (response).</rdfs:comment>
    </owl:Class>
    


    <!-- http://www.w3id.org/hsu-aut/WADL#MatrixParameter -->

    <owl:Class rdf:about="http://www.w3id.org/hsu-aut/WADL#MatrixParameter">
        <rdfs:subClassOf rdf:resource="http://www.w3id.org/hsu-aut/WADL#Parameter"/>
        <rdfs:comment>Specifies a matrix URI component.</rdfs:comment>
    </owl:Class>
    


    <!-- http://www.w3id.org/hsu-aut/WADL#Method -->

    <owl:Class rdf:about="http://www.w3id.org/hsu-aut/WADL#Method">
        <rdfs:subClassOf>
            <owl:Restriction>
                <owl:onProperty rdf:resource="http://www.w3id.org/hsu-aut/WADL#hasRequest"/>
                <owl:maxQualifiedCardinality rdf:datatype="http://www.w3.org/2001/XMLSchema#nonNegativeInteger">1</owl:maxQualifiedCardinality>
                <owl:onClass rdf:resource="http://www.w3id.org/hsu-aut/WADL#Request"/>
            </owl:Restriction>
        </rdfs:subClassOf>
        <rdfs:comment>A method element describes the input to and output from an HTTP protocol method that may be applied to a resource.</rdfs:comment>
    </owl:Class>
    


    <!-- http://www.w3id.org/hsu-aut/WADL#Option -->

    <owl:Class rdf:about="http://www.w3id.org/hsu-aut/WADL#Option">
        <rdfs:comment>An Option element defines one of a set of possible values for the parameter represented by its parent param element.</rdfs:comment>
    </owl:Class>
    


    <!-- http://www.w3id.org/hsu-aut/WADL#PATCH -->

    <owl:Class rdf:about="http://www.w3id.org/hsu-aut/WADL#PATCH">
        <rdfs:subClassOf rdf:resource="http://www.w3id.org/hsu-aut/WADL#Method"/>
        <rdfs:comment>The PATCH method is used to apply partial modifications to a resource.</rdfs:comment>
    </owl:Class>
    


    <!-- http://www.w3id.org/hsu-aut/WADL#POST -->

    <owl:Class rdf:about="http://www.w3id.org/hsu-aut/WADL#POST">
        <rdfs:subClassOf rdf:resource="http://www.w3id.org/hsu-aut/WADL#Method"/>
        <rdfs:comment>The POST method is used to submit an entity to the specified resource, often causing a change in state or side effects on the server.</rdfs:comment>
    </owl:Class>
    


    <!-- http://www.w3id.org/hsu-aut/WADL#PUT -->

    <owl:Class rdf:about="http://www.w3id.org/hsu-aut/WADL#PUT">
        <rdfs:subClassOf rdf:resource="http://www.w3id.org/hsu-aut/WADL#Method"/>
        <rdfs:comment>The PUT method replaces all current representations of the target resource with the request payload.</rdfs:comment>
    </owl:Class>
    


    <!-- http://www.w3id.org/hsu-aut/WADL#Parameter -->

    <owl:Class rdf:about="http://www.w3id.org/hsu-aut/WADL#Parameter">
        <rdfs:comment>A Parameter element describes a parameterized component of its parent element.</rdfs:comment>
    </owl:Class>
    


    <!-- http://www.w3id.org/hsu-aut/WADL#PlainParameter -->

    <owl:Class rdf:about="http://www.w3id.org/hsu-aut/WADL#PlainParameter">
        <rdfs:subClassOf rdf:resource="http://www.w3id.org/hsu-aut/WADL#Parameter"/>
        <rdfs:comment>Specifies a component of the representation formatted as a string encoding of the parameter value according to the rules of the media type.</rdfs:comment>
    </owl:Class>
    


    <!-- http://www.w3id.org/hsu-aut/WADL#QueryParameter -->

    <owl:Class rdf:about="http://www.w3id.org/hsu-aut/WADL#QueryParameter">
        <rdfs:subClassOf rdf:resource="http://www.w3id.org/hsu-aut/WADL#Parameter"/>
        <rdfs:comment>For Resource or Request: Specifies a URI query parameter represented according to the rules for the query component media type specified by the queryType attribute.
For Representation: Specifies a component of the representation as a name value pair formatted according to the rules of the media type. Typically used with media type &apos;application/x-www-form-urlencoded&apos; or &apos;multipart/form-data&apos;.</rdfs:comment>
    </owl:Class>
    


    <!-- http://www.w3id.org/hsu-aut/WADL#Representation -->

    <owl:Class rdf:about="http://www.w3id.org/hsu-aut/WADL#Representation">
        <rdfs:subClassOf>
            <owl:Class>
                <owl:complementOf>
                    <owl:Restriction>
                        <owl:onProperty rdf:resource="http://www.w3id.org/hsu-aut/WADL#hasParameter"/>
                        <owl:someValuesFrom>
                            <owl:Class>
                                <owl:unionOf rdf:parseType="Collection">
                                    <rdf:Description rdf:about="http://www.w3id.org/hsu-aut/WADL#HeaderParameter"/>
                                    <rdf:Description rdf:about="http://www.w3id.org/hsu-aut/WADL#MatrixParameter"/>
                                    <rdf:Description rdf:about="http://www.w3id.org/hsu-aut/WADL#TemplateParameter"/>
                                </owl:unionOf>
                            </owl:Class>
                        </owl:someValuesFrom>
                    </owl:Restriction>
                </owl:complementOf>
            </owl:Class>
        </rdfs:subClassOf>
        <rdfs:comment>A representation element describes a representation of a resource&apos;s state.</rdfs:comment>
    </owl:Class>
    


    <!-- http://www.w3id.org/hsu-aut/WADL#Request -->

    <owl:Class rdf:about="http://www.w3id.org/hsu-aut/WADL#Request">
        <rdfs:subClassOf>
            <owl:Class>
                <owl:complementOf>
                    <owl:Restriction>
                        <owl:onProperty rdf:resource="http://www.w3id.org/hsu-aut/WADL#hasParameter"/>
                        <owl:someValuesFrom>
                            <owl:Class>
                                <owl:unionOf rdf:parseType="Collection">
                                    <rdf:Description rdf:about="http://www.w3id.org/hsu-aut/WADL#MatrixParameter"/>
                                    <rdf:Description rdf:about="http://www.w3id.org/hsu-aut/WADL#PlainParameter"/>
                                    <rdf:Description rdf:about="http://www.w3id.org/hsu-aut/WADL#TemplateParameter"/>
                                </owl:unionOf>
                            </owl:Class>
                        </owl:someValuesFrom>
                    </owl:Restriction>
                </owl:complementOf>
            </owl:Class>
        </rdfs:subClassOf>
        <rdfs:comment>A request element describes the input to be included when applying an HTTP method to a resource.</rdfs:comment>
    </owl:Class>
    


    <!-- http://www.w3id.org/hsu-aut/WADL#Resource -->

    <owl:Class rdf:about="http://www.w3id.org/hsu-aut/WADL#Resource">
        <rdfs:subClassOf>
            <owl:Class>
                <owl:intersectionOf rdf:parseType="Collection">
                    <owl:Restriction>
                        <owl:onProperty rdf:resource="http://www.w3id.org/hsu-aut/WADL#hasMethod"/>
                        <owl:maxQualifiedCardinality rdf:datatype="http://www.w3.org/2001/XMLSchema#nonNegativeInteger">1</owl:maxQualifiedCardinality>
                        <owl:onClass rdf:resource="http://www.w3id.org/hsu-aut/WADL#DELETE"/>
                    </owl:Restriction>
                    <owl:Restriction>
                        <owl:onProperty rdf:resource="http://www.w3id.org/hsu-aut/WADL#hasMethod"/>
                        <owl:maxQualifiedCardinality rdf:datatype="http://www.w3.org/2001/XMLSchema#nonNegativeInteger">1</owl:maxQualifiedCardinality>
                        <owl:onClass rdf:resource="http://www.w3id.org/hsu-aut/WADL#GET"/>
                    </owl:Restriction>
                    <owl:Restriction>
                        <owl:onProperty rdf:resource="http://www.w3id.org/hsu-aut/WADL#hasMethod"/>
                        <owl:maxQualifiedCardinality rdf:datatype="http://www.w3.org/2001/XMLSchema#nonNegativeInteger">1</owl:maxQualifiedCardinality>
                        <owl:onClass rdf:resource="http://www.w3id.org/hsu-aut/WADL#HEAD"/>
                    </owl:Restriction>
                    <owl:Restriction>
                        <owl:onProperty rdf:resource="http://www.w3id.org/hsu-aut/WADL#hasMethod"/>
                        <owl:maxQualifiedCardinality rdf:datatype="http://www.w3.org/2001/XMLSchema#nonNegativeInteger">1</owl:maxQualifiedCardinality>
                        <owl:onClass rdf:resource="http://www.w3id.org/hsu-aut/WADL#PATCH"/>
                    </owl:Restriction>
                    <owl:Restriction>
                        <owl:onProperty rdf:resource="http://www.w3id.org/hsu-aut/WADL#hasMethod"/>
                        <owl:maxQualifiedCardinality rdf:datatype="http://www.w3.org/2001/XMLSchema#nonNegativeInteger">1</owl:maxQualifiedCardinality>
                        <owl:onClass rdf:resource="http://www.w3id.org/hsu-aut/WADL#POST"/>
                    </owl:Restriction>
                    <owl:Restriction>
                        <owl:onProperty rdf:resource="http://www.w3id.org/hsu-aut/WADL#hasMethod"/>
                        <owl:maxQualifiedCardinality rdf:datatype="http://www.w3.org/2001/XMLSchema#nonNegativeInteger">1</owl:maxQualifiedCardinality>
                        <owl:onClass rdf:resource="http://www.w3id.org/hsu-aut/WADL#PUT"/>
                    </owl:Restriction>
                </owl:intersectionOf>
            </owl:Class>
        </rdfs:subClassOf>
        <rdfs:subClassOf>
            <owl:Class>
                <owl:complementOf>
                    <owl:Restriction>
                        <owl:onProperty rdf:resource="http://www.w3id.org/hsu-aut/WADL#hasParameter"/>
                        <owl:someValuesFrom rdf:resource="http://www.w3id.org/hsu-aut/WADL#PlainParameter"/>
                    </owl:Restriction>
                </owl:complementOf>
            </owl:Class>
        </rdfs:subClassOf>
        <rdfs:comment>A resource element describes a set of resources, each identified by a URI that follows a common pattern.</rdfs:comment>
    </owl:Class>
    


    <!-- http://www.w3id.org/hsu-aut/WADL#Resources -->

    <owl:Class rdf:about="http://www.w3id.org/hsu-aut/WADL#Resources">
        <rdfs:comment>The resources element acts as a container for the resources provided by the application.</rdfs:comment>
    </owl:Class>
    


    <!-- http://www.w3id.org/hsu-aut/WADL#Response -->

    <owl:Class rdf:about="http://www.w3id.org/hsu-aut/WADL#Response">
        <rdfs:subClassOf>
            <owl:Class>
                <owl:complementOf>
                    <owl:Restriction>
                        <owl:onProperty rdf:resource="http://www.w3id.org/hsu-aut/WADL#hasParameter"/>
                        <owl:someValuesFrom>
                            <owl:Class>
                                <owl:unionOf rdf:parseType="Collection">
                                    <rdf:Description rdf:about="http://www.w3id.org/hsu-aut/WADL#MatrixParameter"/>
                                    <rdf:Description rdf:about="http://www.w3id.org/hsu-aut/WADL#PlainParameter"/>
                                    <rdf:Description rdf:about="http://www.w3id.org/hsu-aut/WADL#QueryParameter"/>
                                    <rdf:Description rdf:about="http://www.w3id.org/hsu-aut/WADL#TemplateParameter"/>
                                </owl:unionOf>
                            </owl:Class>
                        </owl:someValuesFrom>
                    </owl:Restriction>
                </owl:complementOf>
            </owl:Class>
        </rdfs:subClassOf>
        <rdfs:comment>A response element describes the output that results from performing an HTTP method on a resource.</rdfs:comment>
    </owl:Class>
    


    <!-- http://www.w3id.org/hsu-aut/WADL#TemplateParameter -->

    <owl:Class rdf:about="http://www.w3id.org/hsu-aut/WADL#TemplateParameter">
        <rdfs:subClassOf rdf:resource="http://www.w3id.org/hsu-aut/WADL#Parameter"/>
        <rdfs:comment>The parameter is represented as a string encoding of the parameter value and is substituted into the value of the path attribute of the resource element.</rdfs:comment>
    </owl:Class>
    


    <!-- http://www.w3id.org/hsu-aut/WADL#200 -->

    <owl:Class rdf:about="http://www.w3id.org/hsu-aut/WADL#200">
        <rdfs:subClassOf rdf:resource="http://www.w3id.org/hsu-aut/WADL#Response"/>
        <rdfs:comment>OK: The request was successfully processed and the result of the request is transferred to the response.</rdfs:comment>
    </owl:Class>
    


    <!-- http://www.w3id.org/hsu-aut/WADL#201 -->

    <owl:Class rdf:about="http://www.w3id.org/hsu-aut/WADL#201">
        <rdfs:subClassOf rdf:resource="http://www.w3id.org/hsu-aut/WADL#Response"/>
        <rdfs:comment>Created: The request was successfully processed. The requested resource was created before sending the response. The &quot;location&quot;-header-field may contain the address of the created resource.</rdfs:comment>
    </owl:Class>
    


    <!-- http://www.w3id.org/hsu-aut/WADL#404 -->

    <owl:Class rdf:about="http://www.w3id.org/hsu-aut/WADL#404">
        <rdfs:subClassOf rdf:resource="http://www.w3id.org/hsu-aut/WADL#Response"/>
        <rdfs:comment>Not Found: The requested resource was not found. Also reffered to as dead links.</rdfs:comment>
    </owl:Class>
    


    <!-- http://www.w3id.org/hsu-aut/WADL#500 -->

    <owl:Class rdf:about="http://www.w3id.org/hsu-aut/WADL#500">
        <rdfs:subClassOf rdf:resource="http://www.w3id.org/hsu-aut/WADL#Response"/>
        <rdfs:comment>Internal Server Error: This is a collection status code for unexpected server errors.</rdfs:comment>
    </owl:Class>
    


    <!-- 
    ///////////////////////////////////////////////////////////////////////////////////////
    //
    // General axioms
    //
    ///////////////////////////////////////////////////////////////////////////////////////
     -->

    <rdf:Description>
        <rdf:type rdf:resource="http://www.w3.org/2002/07/owl#AllDisjointClasses"/>
        <owl:members rdf:parseType="Collection">
            <rdf:Description rdf:about="http://www.w3id.org/hsu-aut/WADL#DELETE"/>
            <rdf:Description rdf:about="http://www.w3id.org/hsu-aut/WADL#GET"/>
            <rdf:Description rdf:about="http://www.w3id.org/hsu-aut/WADL#HEAD"/>
            <rdf:Description rdf:about="http://www.w3id.org/hsu-aut/WADL#PATCH"/>
            <rdf:Description rdf:about="http://www.w3id.org/hsu-aut/WADL#POST"/>
            <rdf:Description rdf:about="http://www.w3id.org/hsu-aut/WADL#PUT"/>
        </owl:members>
    </rdf:Description>
    <rdf:Description>
        <rdf:type rdf:resource="http://www.w3.org/2002/07/owl#AllDisjointClasses"/>
        <owl:members rdf:parseType="Collection">
            <rdf:Description rdf:about="http://www.w3id.org/hsu-aut/WADL#HeaderParameter"/>
            <rdf:Description rdf:about="http://www.w3id.org/hsu-aut/WADL#MatrixParameter"/>
            <rdf:Description rdf:about="http://www.w3id.org/hsu-aut/WADL#PlainParameter"/>
            <rdf:Description rdf:about="http://www.w3id.org/hsu-aut/WADL#QueryParameter"/>
            <rdf:Description rdf:about="http://www.w3id.org/hsu-aut/WADL#TemplateParameter"/>
        </owl:members>
    </rdf:Description>
    <rdf:Description>
        <rdf:type rdf:resource="http://www.w3.org/2002/07/owl#AllDisjointClasses"/>
        <owl:members rdf:parseType="Collection">
            <rdf:Description rdf:about="http://www.w3id.org/hsu-aut/WADL#200"/>
            <rdf:Description rdf:about="http://www.w3id.org/hsu-aut/WADL#201"/>
            <rdf:Description rdf:about="http://www.w3id.org/hsu-aut/WADL#404"/>
            <rdf:Description rdf:about="http://www.w3id.org/hsu-aut/WADL#500"/>
        </owl:members>
    </rdf:Description>
</rdf:RDF>



<!-- Generated by the OWL API (version 4.5.9.2019-02-01T07:24:44Z) https://github.com/owlcs/owlapi -->

